added deterministic stuff

Ordered_Resolution_Prover/Deterministic_FO_Ordered_Resolution_Prover.thy
@@ -28,6 +28,12 @@ fun state_of_glstate :: "'a glstate \<Rightarrow> 'a state" where
   "state_of_glstate (N, P, Q, _) =
    (set (map (mset \<circ> fst) N), set (map (mset \<circ> fst) P), set (map (mset \<circ> fst) Q))"
 
+fun is_final_glstate :: "'a glstate \<Rightarrow> bool" where
+  "is_final_glstate (N, P, Q, n) \<longleftrightarrow> N = [] \<and> P = []"
+
+fun is_duplicate_free_glstate where
+  "is_duplicate_free_glstate (N, P, Q, _) \<longleftrightarrow> distinct N \<and> distinct P \<and> distinct Q"
+
 abbreviation rtrancl_resolution_prover_with_weights (infix "\<leadsto>\<^sub>f\<^sup>*" 50) where
   "op \<leadsto>\<^sub>f\<^sup>* \<equiv> (op \<leadsto>\<^sub>f)\<^sup>*\<^sup>*"
 
@@ -143,9 +149,6 @@ fun deterministic_resolution_prover_step :: "'a glstate \<Rightarrow> 'a glstate
           in
             (N, P, Q, n))"
 
-fun is_final_glstate :: "'a glstate \<Rightarrow> bool" where
-  "is_final_glstate (N, P, Q, n) \<longleftrightarrow> N = [] \<and> P = []"
-
 partial_function (option)
   deterministic_resolution_prover :: "'a glstate \<Rightarrow> 'a lclause list option"
 where
@@ -189,6 +192,13 @@ proof (induct C' arbitrary: C)
       using ih[of "L # C"] by simp
   qed
 qed simp
+
+lemma deterministic_resolution_prover_step_duplicate_free:
+  assumes
+    df: "is_duplicate_free_glstate St" and
+    step: "St' = deterministic_resolution_prover_step St"
+  shows "is_duplicate_free_glstate St'"
+  sorry
 
 lemma deterministic_resolution_prover_step_simulation_nonfinal:
   assumes
@@ -243,6 +253,7 @@ proof -
           sorry
       next
         show "(mset C, i) \<notin> set (map (apfst mset) P)"
+          using deterministic_resolution_prover_step_duplicate_free
           sorry
       qed
 
